format-version: 1.2
date: 16:03:2012 09:11
saved-by: antonialock
auto-generated-by: OBO-Edit 2.1-rc3
default-namespace: fission_yeast_phenotype_condition
ontology: fyeco

[Term]
id: FYECO:0000001
name: fission yeast phenotype condition
created_by: antonialock
creation_date: 2012-02-07T11:36:20Z

[Term]
id: FYECO:0000002
name: temperature
def: "The experiment was performed at a specific temperature." []
is_a: FYECO:0000001 ! fission yeast phenotype condition
created_by: antonialock
creation_date: 2012-02-07T12:00:23Z

[Term]
id: FYECO:0000004
name: high temperature
def: "The experiment was performed at a temperature exceeding 32 degrees Celsius." []
is_a: FYECO:0000002 ! temperature
created_by: antonialock
creation_date: 2012-02-07T12:17:29Z

[Term]
id: FYECO:0000005
name: standard temperature
def: "The experiment was performed, or cells were grown, at a temperature within the range 25-32 degrees Celsius." []
synonym: "normal temperature" EXACT []
is_a: FYECO:0000002 ! temperature
disjoint_from: FYECO:0000004 ! high temperature
disjoint_from: FYECO:0000006 ! low temperature
created_by: antonialock
creation_date: 2012-02-07T12:17:29Z

[Term]
id: FYECO:0000006
name: low temperature
def: "The experiment was performed at a temperature lower than 25 degrees Celsius." []
synonym: "cold" EXACT []
is_a: FYECO:0000002 ! temperature
disjoint_from: FYECO:0000004 ! high temperature
created_by: antonialock
creation_date: 2012-02-07T12:17:29Z

[Term]
id: FYECO:0000009
name: growth medium
def: "Any experimental condition specifying the type of growth medium." []
subset: Grouping_terms
is_a: FYECO:0000001 ! fission yeast phenotype condition
created_by: antonialock
creation_date: 2012-02-07T12:28:25Z

[Term]
id: FYECO:0000100
name: medium components
def: "Any experimental condition specifying the nutritional composition of the growth medium." []
comment: Use this term to specify the general type of growth medium. \nIf certain chemicals not normally found in the medium were added, please also use the 'excess chemical added' conditions, for instance 'caffeine added' or 'thiamine added'.\n If a chemical was added in a much lower quantity than normal, please also use the 'limited chemical added' conditions, for instance 'limited adenine added'.
subset: Grouping_terms
synonym: "medium composition" RELATED []
is_a: FYECO:0000009 ! growth medium
created_by: antonialock
creation_date: 2012-05-04T07:48:31Z

[Term]
id: FYECO:0000080
name: rich medium
comment: Use the medium terms to specify the general type of growth medium and its carbon source. \nIf certain chemicals not normally found in the medium were added, please also use the 'chemical added/excluded' terms, for instance 'caffeine added' or 'nitrogen excluded'.\n If a chemical was added in a much lower quantity than normal, please  use the 'limited chemical added' conditions, for instance 'limited adenine added'.
subset: Grouping_terms
is_a: FYECO:0000100 ! medium components
created_by: antonialock
creation_date: 2012-03-14T01:33:58Z

[Term]
id: FYECO:0000137
name: glucose rich medium
def: "Experiments were performed in rich medium  containing glucose as the sole carbon source, yeast extract and other components." []
comment: Use the medium terms to specify the general type of growth medium and its carbon source. \nIf certain chemicals not normally found in the medium were added, please also use the 'chemical added/excluded' terms, for instance 'caffeine added' or 'nitrogen excluded'.\n If a chemical was added in a much lower quantity than normal, please  use the 'limited chemical added' conditions, for instance 'limited adenine added'.
subset: Grouping_terms
is_a: FYECO:0000080 ! rich medium
created_by: antonialock
creation_date: 2012-06-14T20:35:20Z

[Term]
id: FYECO:0000012
name: standard glucose rich medium
def: "Experiments were performed in rich medium containing yeast extract and other components. The concentration of glucose is typically around 2-3%." []
comment: Use the medium terms to specify the general type of growth medium and its carbon source. \nIf certain chemicals not normally found in the medium were added, please also use the 'chemical added/excluded' terms, for instance 'caffeine added' or 'nitrogen excluded'.\n If a chemical was added in a much lower quantity than normal, please  use the 'limited chemical added' conditions, for instance 'limited adenine added'.
synonym: "YE" BROAD []
synonym: "YES" EXACT []
is_a: FYECO:0000137 ! glucose rich medium
created_by: antonialock
creation_date: 2012-02-07T12:39:25Z

[Term]
id: FYECO:0000138
name: glycerol YE
alt_id: FYECO:0000083
def: "Experiments were performed in rich medium containing glycerol as the sole carbon source, yeast extract and other components. The concentration of glycerol is typically around 2-3% and supplemented with trace amounts of another carbon source (e.g. glucose)." [PomBase:al]
comment: Use the medium terms to specify the general type of growth medium and its carbon source. If certain chemicals not normally found in the medium were added, please also use the 'chemical added/excluded' terms, such as 'caffeine added' or 'nitrogen excluded'. If a chemical was added in a much lower quantity than normal, please use the 'limited chemical added' conditions, for instance 'limited adenine added'.
synonym: "glycerol rich medium" BROAD [PomBase:al]
synonym: "glycerol sole carbon source rich medium" EXACT [PomBase:al]
synonym: "glycerol sole carbon source YE" RELATED [PomBase:al]
is_obsolete: true
is_a: FYECO:0000080 ! grouping rich medium
created_by: antonialock
creation_date: 2012-06-14T20:38:23Z

[Typedef]
id: part_of
name: part_of
xref: OBO_REL:part_of
created_by: antonialock
creation_date: 2012-02-07T11:57:34Z

